Strata/Languages/Core/FactoryWF.lean
@@ -20,4 +20,6 @@ namespace Core
 
 public theorem Factory_wf : Lambda.FactoryWF Factory := by simp [Factory]
 
+public theorem Factory_closed : Lambda.FactoryClosed Factory := by simp [Factory]
+
 end Core
